Add locations to input and output of lexer (#6)

Veriflex/Lexer.lean
@@ -2,6 +2,7 @@ import Veriflex.Grammar
 import Veriflex.Brzozowski
 import Veriflex.Utils
 import Veriflex.MaxPrefix
+import Veriflex.Located
 
 /-!
 # Lexer
@@ -11,26 +12,29 @@ This file implements the function `lex` which takes a grammar and lexes a string
 namespace Veriflex
 
 def apply_rule  {tok : Type} :
-  Rule tok × Option (List Char × List Char) →
-  Option (tok × Nat × List Char) := λ ⟨rule,x ⟩ =>
+  Rule tok × Option (List LChar × List LChar) →
+  Option (tok × List LChar × List LChar) := λ ⟨rule,x ⟩ =>
   match x with
   | none => none
-  | some ⟨pre, rest⟩ => some ⟨rule.action (String.mk pre), pre.length, rest⟩
+  | some ⟨pre, rest⟩ => some ⟨rule.action (String.mk (contents pre)), pre, rest⟩
 
-def max_pref {tok : Type}(input : List Char) (rules : List (Rule tok)) : Option (tok × Nat × List Char) :=
-  let max_prefixes : List (Rule tok × Option (List Char × List Char)) := rules.map (λ rule => ⟨rule, max_pref_one rule.re input⟩)
-  let max_prefixes : List (Option (tok × Nat × List Char)) := max_prefixes.map apply_rule
-  let max_prefixes : List (tok × Nat × List Char) := max_prefixes.filterMap id
-  let result : Option (tok × Nat × List Char):= find_first_max max_prefixes (λ x => x.2.1)
+def max_pref {tok : Type}
+             (input : List LChar)
+             (G : Grammar tok)
+             : Option (tok × List LChar × List LChar) :=
+  let max_prefixes : List (Rule tok × Option (List LChar × List LChar)) := G.map (λ rule => ⟨rule, max_pref_one rule.re input⟩)
+  let max_prefixes : List (Option (tok × List LChar × List LChar)) := max_prefixes.map apply_rule
+  let max_prefixes : List (tok × List LChar × List LChar) := max_prefixes.filterMap id
+  let result : Option (tok × List LChar × List LChar):= find_first_max max_prefixes (λ x => x.2.1.length)
   result
 
 theorem max_pref_length :
-  max_pref input rules = some ⟨tok,n,rest⟩ →
-  input.length = n + rest.length := by
+  max_pref input rules = some ⟨tok,pre,rest⟩ →
+  input.length = pre.length + rest.length := by
   unfold max_pref
   simp!
   generalize H_eq : List.filterMap (apply_rule ∘ fun rule => (rule, max_pref_one rule.re input)) rules = xs
-  have H_forall : ∀ x ∈ xs, input.length = x.snd.fst + x.snd.snd.length := by
+  have H_forall : ∀ x ∈ xs, input.length = x.snd.fst.length + x.snd.snd.length := by
     intros x H_in
     rw [←H_eq] at H_in
     let ⟨tok,n,rest⟩ := x
@@ -51,20 +55,24 @@ theorem max_pref_length :
       rw [List.length_append]
   intros H
   have H_in := find_first_max_contained H
-  specialize H_forall ⟨ tok,n ,rest⟩ H_in
+  specialize H_forall ⟨ tok,pre ,rest⟩ H_in
   assumption
 
-def first_token {tok : Type}(input : List Char) (rules : List (Rule tok)) : Option (tok × List Char) :=
-  match max_pref input rules with
+def first_token {tok : Type}
+                (G : Grammar tok)
+                (input : List LChar)
+                : Option (Located tok × List LChar) :=
+  match max_pref input G with
   | none => none
-  | some ⟨tok,n,rest⟩ => if n > 0
-                         then some ⟨tok, rest⟩
-                         else none
+  | some ⟨tok,pre,rest⟩ =>
+    match pre with
+    | List.nil => none
+    | List.cons x _ => some ⟨Located.mk x.location tok, rest⟩
 
 
 
 theorem first_token_smaller :
-  first_token input rules = some ⟨tok, rest⟩ →
+  first_token rules input = some ⟨tok, rest⟩ →
   rest.length < input.length := by
   unfold first_token
   generalize H_eq : max_pref input rules = res
@@ -75,29 +83,39 @@ theorem first_token_smaller :
   | some v =>
     let ⟨token,n,rest'⟩ := v
     simp! at H
-    have X : input.length = n + rest'.length := by
+    have X : input.length = n.length + rest'.length := by
       apply max_pref_length
       apply H_eq
-    let ⟨H₁,_,H₂⟩ := H
-    rw [X,H₂]
-    omega
+    clear H_eq
+    cases n with
+    | nil => simp! at H
+    | cons hd tl =>
+      simp! at H
+      let ⟨H₁,H₂⟩ := H
+      simp! at X
+      rw [H₂] at X
+      omega
 
-def measure (x : Option (tok × List Char)) : Nat :=
+def measure {tok a : Type}(x : Option (tok × List a)) : Nat :=
   match x with
   | none => 0
   | some ⟨ _, xs ⟩ => xs.length + 1
 
-def lex_rec {tok : Type}(input : List Char)(foo: Option (tok × List Char))(rules : List (Rule tok)) : List tok × List Char :=
-  match foo with
+def lex_rec {tok : Type}
+            (G : Grammar tok)
+            (input : List LChar)
+            (next: Option (Located tok × List LChar))
+            : List (Located tok) × List LChar :=
+  match next with
   | none => ([], input)
   | some (tok, rest) =>
     let (toks, rest') :=
-      lex_rec rest (first_token rest rules) rules
+      lex_rec G rest (first_token G rest)
     (tok :: toks, rest')
-termination_by measure foo
+termination_by measure next
 decreasing_by
   simp!
-  generalize H : first_token rest rules = x
+  generalize H : first_token G rest = x
   cases x with
   | none =>
     simp!
@@ -106,7 +124,10 @@ decreasing_by
     simp!
     exact (first_token_smaller H)
 
-def lex {tok : Type}(input : List Char) (rules : List (Rule tok)) : List tok × List Char :=
-  lex_rec input (first_token input rules) rules
+def lex {tok : Type}
+        (G : Grammar tok)
+        (input : List LChar)
+        : List (Located tok) × List LChar :=
+  lex_rec G input (first_token G input)
 
 end Veriflex
