Veriflex/Example.lean
@@ -128,16 +128,21 @@ Note that the order of the rules is important:
 expressions match the string "data", but this string should be lexed as
 a keyword, not an identifier.
 -/
-def grammar : List (Rule Token) :=
+def grammar : Grammar Token :=
   [KeywordData, Identifier, IntLiteral, Whitespace]
 
-def lexer (s : String) : List Token :=
-  (lex s.toList grammar).fst
+def columnize (s : String) : List LChar :=
+ s.toList.zipIdx.map (λ ⟨c,l⟩ => Located.mk l c)
 
-#guard lexer "data" == [Token.KeywordData]
-#guard lexer "foo" == [Token.Identifier "foo"]
-#guard lexer "123" == [Token.IntLiteral 123]
-#guard lexer "  " == [Token.Whitespace]
-#guard lexer "123 foo" == [Token.IntLiteral 123, Token.Whitespace, Token.Identifier "foo"]
+def lexer (s : String) : List (Located Token) :=
+  (lex grammar (columnize s)).fst
+
+#guard lexer "data"    == [ Located.mk 0 Token.KeywordData ]
+#guard lexer "foo"     == [ Located.mk 0 (Token.Identifier "foo") ]
+#guard lexer "123"     == [ Located.mk 0 (Token.IntLiteral 123) ]
+#guard lexer "  "      == [ Located.mk 0 Token.Whitespace ]
+#guard lexer "123 foo" == [ Located.mk 0 (Token.IntLiteral 123)
+                          , Located.mk 3 Token.Whitespace
+                          , Located.mk 4 (Token.Identifier "foo") ]
 
 end Veriflex
