Veriflex/Located.lean
@@ -1,0 +1,28 @@
+/-!
+# Located
+
+This file defines a structure `Located` that is used to track source code locations of
+characters and tokens, as well as utility functions.
+-/
+namespace Veriflex
+
+abbrev Location : Type := Nat
+
+structure Located (a : Type) : Type where
+  location : Location
+  content : a
+  deriving BEq
+
+abbrev LChar : Type := Located Char
+
+/-- Forget the locations and return the -/
+def contents {a : Type} (xs : List (Located a)) : List a :=
+  xs.map (λ x => x.content)
+
+/-- Returns the location of the first item in the list, if it exists. -/
+def first_loc {a : Type} (xs : List (Located a)) : Option Location :=
+  match xs with
+  | List.nil => none
+  | List.cons x _ => some x.location
+
+end Veriflex
